\documentclass{article}
\usepackage{amsmath}
\usepackage{amsthm}
\usepackage{amssymb}
\usepackage{enumerate}
\begin{document}
We have proved  $ C(A)=C(A^T),N(A)=N(A^T) $, so there exsts a invertible  $ P \in GL_n(K)$, such that  $ A=PA^T $,
then  $ A^T=(PA^T)^T=AP^T $.

Then  $ A^2=AA^T $ implies  $ A^2=AAP^T\Rightarrow A^2(I_n-P^T)=0 $ which implies $ A(I_n-P^T)=0 $ ( for  $  N(A^2)=N(AA^T)=N(A^T)=N(A) $ ).

i.e. $ A=AP^T=A^T $ 

Similar for $ A^2=-AA^T $( replace  $ I_n-P^T $ to  $ I_n+P^T $  ) 
\end{document}